[ACL2s] Updated cgen so that it supports a new parameter, single-test-timeout. The default value is 1/100 and it determines how long cgen spends on testing a singe test. This is useful when you have functions that can be slow on some inputs, e.g., fib. Without this flag, if cgen tried fib on 100, that consumed the whole testing time budget. Now, it will only consume 1/100 of a second. Timeouts are treated as vacuous tests by cgen for data collection and reporting purposes. I'll change that once we have more experience with the new parameter.
I also had to commit updates to defdata to allow for more flexible enumeration, but while
that seems stable, it is still a work in progress, so more on that later.

books/acl2s/defdata/base.lisp
@@ -406,10 +406,75 @@ on a per data definition basis or
   (let ((range (- hi lo)))
     (+ lo (simple-hash n range))))
 
+(local (include-book "arithmetic-5/top" :dir :system))
+       
+(defun bitsize-aux (n acc)
+  (declare (xargs :guard (and (natp n) (posp acc))))
+  (if (and (integerp n) (> n 1))
+      (bitsize-aux (floor (nfix n) 2) (1+ acc))
+    acc))
+
+(defthm bitsize-aux-posp
+  (implies (and (natp n) (posp acc))
+           (posp (bitsize-aux n acc))))
+
+(defun bitsize (n)
+  (declare (xargs :guard (natp n)))
+  (bitsize-aux n 1))
+
+; (bitsize 0)
+; (bitsize 1)
+; (bitsize 63)
+; (bitsize 64)
+
+(defun rounds (lo hi stop-bits)
+  (declare (xargs :guard (and (integerp lo)
+                              (integerp hi)
+                              (<= lo hi)
+                              (posp stop-bits))))
+  (let* ((range (nfix (- hi lo)))
+         (size (bitsize range)))
+    (if (<= size stop-bits)
+        1
+      (- size (1- stop-bits)))))
+    
+; (rounds 0 1023 10)
+; (rounds 0 1024 10)
+
+(defun nth-integer-between-bits-mid (n lo hi bits)
+  (declare (xargs :guard (and (natp n)
+                              (integerp lo)
+                              (integerp hi)
+                              (<= lo hi)
+                              (posp bits))))
+  (let* ((fullrange (- hi lo))
+         (brange (min fullrange (1- (expt 2 bits))))
+         (fullmid (+ lo (floor fullrange 2)))
+         (blo (- fullmid (floor brange 2))))
+    (+ blo (simple-hash n brange))))
+
+(defun nth-integer-between-bits-lo (n lo hi bits)
+  (declare (xargs :guard (and (natp n)
+                              (integerp lo)
+                              (integerp hi)
+                              (<= lo hi)
+                              (posp bits))))
+  (let* ((fullrange (- hi lo))
+         (brange (min fullrange (1- (expt 2 bits)))))
+    (+ lo (simple-hash n brange))))
+
+;(nth-integer-between-bits-mid 1021312 0 10000 100)
+;(nth-integer-between-bits-lo  1021312 0 10000 100)
+;(nth-integer-between          1021312 0 10000)
+
+;(nth-integer-between-bits-mid 1021312 0 10000 8)
+;(nth-integer-between-bits-lo  1021312 0 10000 8)
+;(nth-integer-between          1021312 0 10000)
+
 (defun integer-index (i)
   (declare (xargs :guard (integerp i)))
   (if (< i 0)
-    (1+ (* (- (1+ i)) 2))
+      (1+ (* (- (1+ i)) 2))
     (* i 2)))
 
 #|
@@ -834,7 +899,6 @@ as a type.
     (complex-rational (nth-complex-rational-between n lo hi))
     (t (nth-acl2-number-between n lo hi))))
   
-
 (defmacro nth-number-between (n lo hi &key type)
   `(nth-number-between-fn ,n ,lo ,hi (or ,type 'acl2s::acl2-number)))
 
